src/Std/Data/DTreeMap/Internal/Queries.lean
@@ -26,7 +26,7 @@ private local instance : Coe (Type v) (α → Type v) where coe γ := fun _ => �
 
 namespace Std.DTreeMap.Internal.Impl
 
-/-- Two hash maps are equivalent in the sense of Equiv iff all the keys and values are equal. -/
+/-- Two tree maps are equivalent in the sense of Equiv iff all the keys and values are equal. -/
 structure Equiv (t t' : Impl α β) where
   /-- Implementation detail of the tree map -/
   impl : t.toListModel.Perm t'.toListModel
